Progress towards factoring backend/proofs
In particular create a word_gcFunctions theory to house a bunch of
definitions and minor theorems used by a number of ...Proof scripts.
Rather than have these in one of the Proof files, moving them into
their own separate file lets the Proof files run concurrently and
doesn't misrepresent the conceptual dependency story.

compiler/backend/proofs/data_to_word_assignProofScript.sml
@@ -5,13 +5,15 @@ open preamble bvlSemTheory dataSemTheory dataPropsTheory
      labPropsTheory whileTheory set_sepTheory semanticsPropsTheory
      helperLib alignmentTheory blastLib
      word_bignumTheory wordLangTheory word_bignumProofTheory
-     gen_gc_partialTheory gc_sharedTheory;
+     gen_gc_partialTheory gc_sharedTheory word_gcFunctionsTheory;
 local open gen_gcTheory in end
 
 val _ = new_theory "data_to_word_assignProof";
 
 val _ = hide "next";
 val shift_def = backend_commonTheory.word_shift_def
+val isWord_def = wordSemTheory.isWord_def
+val theWord_def = wordSemTheory.theWord_def
 
 val _ = temp_overload_on("FALSE_CONST",``Const (n2w 2:'a word)``)
 val _ = temp_overload_on("TRUE_CONST",``Const (n2w 18:'a word)``)
